src/ldrfra/PFtoAPFSimThread.v
@@ -22,11 +22,13 @@ Require Import Local.
 Require Import Thread.
 
 Require Import MemoryMerge.
+Require Import MemoryReorder.
 
 Require Import PFStep.
 Require Import OrdStep.
-Require Import RelWrites.
-Require Import RelStep.
+Require Import Writes.
+Require Import WStep.
+Require Import Stable.
 
 Set Implicit Arguments.
 
@@ -36,24 +38,28 @@ Module PFtoAPFSimThread.
     Variable lang: language.
     Variable L: Loc.t -> bool.
 
-    Variant sim_memory (rels: RelWrites.t) (mem_src mem_tgt: Memory.t): Prop :=
+    Variant sim_memory (rels: Writes.t) (mem_src mem_tgt: Memory.t): Prop :=
     | sim_memory_intro
         (SOUND: Memory.le mem_src mem_tgt)
-        (COMPLETE1: forall loc (LOC: L loc), Cell.le (mem_tgt loc) (mem_src loc))
+        (COMPLETE1: forall loc (LOC: ~ L loc)
+                      from to msg (GET_TGT: Memory.get loc to mem_tgt = Some (from, msg)),
+            (<<GET_SRC: Memory.get loc to mem_src = Some (from, msg)>>))
         (COMPLETE2: forall loc ts from to msg
-                      (LOC: ~ L loc) (LE: Time.le ts to)
+                      (LOC: L loc) (LE: Time.le ts to)
                       (GET_TGT: Memory.get loc to mem_tgt = Some (from, msg)),
             (<<GET_SRC: Memory.get loc to mem_src = Some (from, msg)>>) \/
-            exists from' to' val released,
+            exists from' to' val ord,
+              (<<IN: List.In (loc, to', ord) rels>>) /\
               (<<LT: Time.lt ts to'>>) /\
-              (<<GET_SRC: Memory.get loc to' mem_src = Some (from', Message.concrete val released)>>))
+              (<<ORD: Ordering.le ord Ordering.na>>) /\
+              (<<GET_SRC: Memory.get loc to' mem_src = Some (from', Message.concrete val None)>>))
         (RESERVE: forall loc from to
                     (GET_TGT: Memory.get loc to mem_tgt = Some (from, Message.reserve)),
             (<<GET_SRC: Memory.get loc to mem_src = Some (from, Message.reserve)>>))
     .
     Hint Constructors sim_memory.
 
-    Inductive sim_statelocal (rels: RelWrites.t):
+    Inductive sim_statelocal (rels: Writes.t):
       forall (sl_src sl_tgt: {lang : language & Language.state lang} * Local.t), Prop :=
     | sim_statelocal_intro
         lang st lc_src lc_tgt
@@ -62,14 +68,675 @@ Module PFtoAPFSimThread.
     .
     Hint Constructors sim_statelocal.
 
-    Inductive sim_thread (rels: RelWrites.t) (e_src e_tgt: Thread.t lang): Prop :=
+    Inductive sim_thread (rels: Writes.t) (e_src e_tgt: Thread.t lang): Prop :=
     | sim_thread_intro
         (STATE: (Thread.state e_src) = (Thread.state e_tgt))
         (LOCAL: (Thread.local e_src) = (Thread.local e_tgt))
-        (PROMISES: OrdLocal.reserve_only L (Local.promises (Thread.local e_src)))
+        (* (RESERVE_ONLY: OrdLocal.reserve_only L (Local.promises (Thread.local e_src))) *)
+        (* (WRITES_WF: Writes.wf rels (Local.promises (Thread.local e_src)) (Thread.memory e_src)) *)
         (SC: (Thread.sc e_src) = (Thread.sc e_tgt))
         (MEMORY: sim_memory rels (Thread.memory e_src) (Thread.memory e_tgt))
     .
     Hint Constructors sim_thread.
+
+    Lemma sim_memory_cons
+          a rels mem_src mem_tgt
+          (MEM: sim_memory rels mem_src mem_tgt):
+      sim_memory (a :: rels) mem_src mem_tgt.
+    Proof.
+      inv MEM. econs; eauto. i.
+      exploit COMPLETE2; eauto. i. des; eauto.
+      right. esplits; eauto. econs 2. ss.
+    Qed.
+
+    Lemma sim_memory_append
+          e rels mem_src mem_tgt
+          (MEM: sim_memory rels mem_src mem_tgt):
+      sim_memory (Writes.append L e rels) mem_src mem_tgt.
+    Proof.
+      unfold Writes.append.
+      destruct e; ss; condtac; ss; apply sim_memory_cons; ss.
+    Qed.
+
+    Lemma sim_memory_app
+          rels' rels mem_src mem_tgt
+          (MEM: sim_memory rels mem_src mem_tgt):
+      sim_memory (rels' ++ rels) mem_src mem_tgt.
+    Proof.
+      inv MEM. econs; eauto. i.
+      exploit COMPLETE2; eauto. i. des; eauto.
+      right. esplits; eauto.
+      apply List.in_or_app. eauto.
+    Qed.
+
+    Lemma promise
+          rels mem1_src
+          promises1 mem1_tgt loc from to msg promises2 mem2_tgt kind
+          (MEM1: sim_memory rels mem1_src mem1_tgt)
+          (WRITES1: Writes.wf L rels mem1_src)
+          (LE1_SRC: Memory.le promises1 mem1_src)
+          (PROMISE_TGT: Memory.promise promises1 mem1_tgt loc from to msg promises2 mem2_tgt kind):
+      exists mem2_src,
+        <<PROMISE_SRC: Memory.promise promises1 mem1_src loc from to msg promises2 mem2_src kind>> /\
+        <<MEM2: sim_memory rels mem2_src mem2_tgt>>.
+    Proof.
+      inv MEM1. inv PROMISE_TGT; ss.
+      { (* add *)
+        exploit (@Memory.add_exists mem1_src loc from to msg).
+        { i. exploit SOUND; eauto. i.
+          exploit Memory.add_get0; try exact MEM. i. des.
+          exploit Memory.add_get1; try exact x; eauto. i.
+          exploit Memory.get_disjoint; [exact GET0|exact x1|]. i. des; subst; ss. congr.
+        }
+        { inv MEM. inv ADD. ss. }
+        { inv MEM. inv ADD. ss. }
+        i. des. esplits; eauto. econs; ii.
+        - erewrite Memory.add_o; eauto.
+          revert LHS. erewrite Memory.add_o; try exact x0.
+          condtac; ss; eauto.
+        - erewrite Memory.add_o; eauto.
+          revert GET_TGT. erewrite Memory.add_o; try exact MEM.
+          condtac; ss; eauto.
+        - revert GET_TGT. erewrite Memory.add_o; try exact MEM.
+          condtac; ss.
+          + i. des. clarify.
+            exploit Memory.add_get0; try exact x0. i. des. eauto.
+          + guardH o. i. exploit COMPLETE2; eauto. i. des.
+            * exploit Memory.add_get1; try exact GET_SRC; eauto.
+            * exploit Memory.add_get1; try exact GET_SRC; eauto. i.
+              right. esplits; try exact x1; eauto.
+        - erewrite Memory.add_o; eauto.
+          revert GET_TGT. erewrite Memory.add_o; try exact MEM.
+          condtac; ss; eauto.
+      }
+
+      { (* split *)
+        exploit Memory.split_exists_le; try exact LE1_SRC; eauto. i. des.
+        esplits; eauto. econs; ii.
+        - erewrite Memory.split_o; eauto.
+          revert LHS. erewrite Memory.split_o; try exact x0.
+          repeat condtac; ss; eauto.
+        - erewrite Memory.split_o; eauto.
+          revert GET_TGT. erewrite Memory.split_o; try exact MEM.
+          repeat condtac; ss; eauto.
+        - revert GET_TGT. erewrite Memory.split_o; try exact MEM.
+          repeat condtac; ss.
+          + i. des. clarify.
+            exploit Memory.split_get0; try exact x0. i. des. eauto.
+          + guardH o. i. des. clarify.
+            exploit Memory.split_get0; try exact x0. i. des. eauto.
+          + guardH o. guardH o0.
+            i. exploit COMPLETE2; eauto. i. des.
+            * left. erewrite Memory.split_o; eauto. repeat condtac; ss; congr.
+            * exploit Memory.split_get1; try exact GET_SRC; eauto. i. des.
+              right. esplits; eauto.
+        - erewrite Memory.split_o; eauto.
+          revert GET_TGT. erewrite Memory.split_o; try exact MEM.
+          repeat condtac; ss; eauto.
+      }
+
+      { (* lower *)
+        exploit Memory.lower_exists_le; try exact LE1_SRC; eauto. i. des.
+        esplits; eauto. econs; ii.
+        - erewrite Memory.lower_o; eauto.
+          revert LHS. erewrite Memory.lower_o; try exact x0.
+          condtac; ss; eauto.
+        - erewrite Memory.lower_o; eauto.
+          revert GET_TGT. erewrite Memory.lower_o; try exact MEM.
+          condtac; ss; eauto.
+        - revert GET_TGT. erewrite Memory.lower_o; try exact MEM.
+          condtac; ss.
+          + i. des. clarify.
+            exploit Memory.lower_get0; try exact x0. i. des. eauto.
+          + guardH o. i. exploit COMPLETE2; eauto. i. des.
+            * left. erewrite Memory.lower_o; eauto. condtac; ss; eauto.
+            * exploit Memory.lower_get1; try exact GET_SRC; eauto. i. des.
+              inv MSG_LE. inv RELEASED.
+              right. esplits; eauto.
+        - erewrite Memory.lower_o; eauto.
+          revert GET_TGT. erewrite Memory.lower_o; try exact MEM.
+          condtac; ss; eauto.
+      }
+
+      { (* remove *)
+        exploit Memory.remove_exists_le; try exact LE1_SRC; eauto. i. des.
+        esplits; eauto. econs; ii.
+        - erewrite Memory.remove_o; eauto.
+          revert LHS. erewrite Memory.remove_o; try exact x0.
+          condtac; ss; eauto.
+        - erewrite Memory.remove_o; eauto.
+          revert GET_TGT. erewrite Memory.remove_o; try exact MEM.
+          condtac; ss; eauto.
+        - revert GET_TGT. erewrite Memory.remove_o; try exact MEM.
+          condtac; ss.
+          guardH o. i. exploit COMPLETE2; eauto. i. des.
+          + left. erewrite Memory.remove_o; eauto. condtac; ss; eauto.
+          + exploit Memory.remove_get1; try exact GET_SRC; eauto. i. des.
+            { subst. exploit Memory.remove_get0; try exact x0. i. des. congr. }
+            right. esplits; eauto.
+        - erewrite Memory.remove_o; eauto.
+          revert GET_TGT. erewrite Memory.remove_o; try exact MEM.
+          condtac; ss; eauto.
+      }
+    Qed.
+
+    Lemma write
+          rels mem1_src
+          promises1 mem1_tgt loc from to msg promises2 mem2_tgt kind
+          (MEM1: sim_memory rels mem1_src mem1_tgt)
+          (WRITES1: Writes.wf L rels mem1_src)
+          (LE1_SRC: Memory.le promises1 mem1_src)
+          (WRITE_TGT: Memory.write promises1 mem1_tgt loc from to msg promises2 mem2_tgt kind):
+      exists mem2_src,
+        <<WRITE_SRC: Memory.write promises1 mem1_src loc from to msg promises2 mem2_src kind>> /\
+        <<MEM2: sim_memory rels mem2_src mem2_tgt>>.
+    Proof.
+      inv WRITE_TGT. exploit promise; eauto. i. des.
+      esplits; eauto.
+    Qed.
+
+    Lemma write_na_other
+          rels mem1_src
+          ts promises1 mem1_tgt loc from to val promises2 mem2_tgt msgs kinds kind
+          (MEM1: sim_memory rels mem1_src mem1_tgt)
+          (WRITES1: Writes.wf L rels mem1_src)
+          (LE1_SRC: Memory.le promises1 mem1_src)
+          (LOC: ~ L loc)
+          (WRITE_TGT: Memory.write_na ts promises1 mem1_tgt loc from to val promises2 mem2_tgt msgs kinds kind):
+      exists mem2_src,
+        <<WRITE_SRC: Memory.write_na ts promises1 mem1_src loc from to val promises2 mem2_src msgs kinds kind>> /\
+        <<MEM2: sim_memory rels mem2_src mem2_tgt>>.
+    Proof.
+      revert mem1_src MEM1 WRITES1 LE1_SRC.
+      induction WRITE_TGT; i.
+      { exploit write; eauto. i. des. eauto. }
+      exploit write; eauto. i. des.
+      hexploit Memory.write_le; try exact WRITE_SRC; eauto. i.
+      hexploit Writes.write_wf_other; try exact WRITE_SRC; eauto. i.
+      exploit IHWRITE_TGT; try exact MEM2; eauto. i. des.
+      esplits; eauto.
+    Qed.
+
+    Lemma write_add_memory_add
+          promises1 mem1 loc from to msg promises2 mem2
+          (WRITE: Memory.write promises1 mem1 loc from to msg promises2 mem2 Memory.op_kind_add):
+      (<<PROMISES: promises2 = promises1>>) /\
+      (<<ADD: Memory.add mem1 loc from to msg mem2>>).
+    Proof.
+      inv WRITE. inv PROMISE. splits; ss.
+      exploit MemoryMerge.add_remove; try exact PROMISES; eauto.
+    Qed.
+
+    Lemma reorder_add_write_add
+          promises0 mem0 loc from1 to1 msg1 mem1
+          from2 to2 msg2 promises2 mem2
+          (ADD: Memory.add mem0 loc from1 to1 msg1 mem1)
+          (WRITE: Memory.write promises0 mem1 loc from2 to2 msg2 promises2 mem2 Memory.op_kind_add):
+      exists mem1',
+        (<<WRITE: Memory.write promises0 mem0 loc from2 to2 msg2 promises2 mem1' Memory.op_kind_add>>) /\
+        (<<ADD: Memory.add mem1' loc from1 to1 msg1 mem2>>).
+    Proof.
+      inv WRITE. inv PROMISE.
+      exploit MemoryReorder.add_add; [exact ADD|exact MEM|]. i. des.
+      exploit MemoryMerge.add_remove; [exact PROMISES|exact REMOVE|]. i. subst.
+      esplits; try exact ADD2.
+      econs; [econs; eauto|]; eauto. i.
+      exploit Memory.add_get1; try exact ADD; eauto.
+    Qed.
+
+    Lemma reserve_only_write_add
+          promises1 mem1 loc from to msg promises2 mem2 kind
+          (RESERVE_ONLY: OrdLocal.reserve_only L promises1)
+          (LOC: L loc)
+          (WRITE: Memory.write promises1 mem1 loc from to msg promises2 mem2 kind):
+      kind = Memory.op_kind_add.
+    Proof.
+      inv WRITE. inv PROMISE; ss; exfalso.
+      - exploit Memory.split_get0; try exact PROMISES. i. des. eauto.
+      - exploit Memory.lower_get0; try exact PROMISES. i. des.
+        exploit RESERVE_ONLY; eauto. i. subst. inv MSG_LE. ss.
+      - exploit Memory.remove_get0; try exact PROMISES. i. des.
+        exploit Memory.remove_get0; try exact REMOVE. i. des. congr.
+    Qed.
+
+    Lemma reorder_write_write_na
+          promises0 mem0 loc from1 to1 msg1 promises1 mem1 kind1
+          ts from2 to2 val2 promises2 mem2 msgs2 kinds2 kind2
+          (RESERVE_ONLY: OrdLocal.reserve_only L promises0)
+          (LOC: L loc)
+          (WRITE: Memory.write promises0 mem0 loc from1 to1 msg1 promises1 mem1 kind1)
+          (WRITE_NA: Memory.write_na ts promises1 mem1 loc from2 to2 val2 promises2 mem2 msgs2 kinds2 kind2):
+      exists mem1',
+        (<<WRITE_NA: Memory.write_na ts promises0 mem0 loc from2 to2 val2 promises2 mem1' msgs2 kinds2 kind2>>) /\
+        (<<ADD: Memory.add mem1' loc from1 to1 msg1 mem2>>).
+    Proof.
+      exploit reserve_only_write_add; eauto. i. subst.
+      exploit write_add_memory_add; eauto. i. des. subst.
+      clear WRITE. revert ts mem0 mem1 promises2 mem2 kinds2 ADD WRITE_NA.
+      induction msgs2 as [|[to' msg'] msgs]; i.
+      { inv WRITE_NA.
+        exploit reserve_only_write_add; eauto. i. subst.
+        exploit reorder_add_write_add; eauto. i. des.
+        esplits; eauto.
+      }
+      inv WRITE_NA.
+      hexploit OrdLocal.write_reserve_only; try exact WRITE_EX; eauto. i.
+      exploit reserve_only_write_add; try exact WRITE_EX; eauto. i. subst.
+      exploit reorder_add_write_add; try exact ADD; eauto. i. des.
+      exploit write_add_memory_add; try exact WRITE_EX. i. des. subst. clear ADD1.
+      exploit IHmsgs; try exact ADD0; try exact WRITE_NA0. i. des.
+      esplits; eauto.
+    Qed.
+
+    Lemma write_na_loc
+          rels mem1_src
+          ts promises1 mem1_tgt loc from to val promises2 mem2_tgt msgs kinds kind
+          ord
+          (MEM1: sim_memory rels mem1_src mem1_tgt)
+          (WRITES1: Writes.wf L rels mem1_src)
+          (RESERVE_ONLY: OrdLocal.reserve_only L promises1)
+          (LE1_SRC: Memory.le promises1 mem1_src)
+          (LOC: L loc)
+          (ORD: Ordering.le ord Ordering.na)
+          (WRITE_TGT: Memory.write_na ts promises1 mem1_tgt loc from to val promises2 mem2_tgt msgs kinds kind):
+      exists mem2_src,
+        (<<WRITE_SRC: Memory.write promises1 mem1_src loc from to (Message.concrete val None) promises2 mem2_src kind>>) /\
+        (<<MEM2: sim_memory ((loc, to, ord) :: rels) mem2_src mem2_tgt>>).
+    Proof.
+      revert ts mem1_tgt promises2 mem2_tgt kinds MEM1 WRITE_TGT.
+      induction msgs as [|[to' msg'] msgs]; i.
+      { inv WRITE_TGT.
+        exploit write; eauto. i. des.
+        esplits; eauto using sim_memory_cons.
+      }
+      inv WRITE_TGT.
+      exploit reserve_only_write_add; try exact WRITE_EX; eauto. i. subst.
+      exploit reorder_write_write_na; eauto. i. des.
+      exploit IHmsgs; try exact WRITE_NA0; eauto. i. des.
+      esplits; eauto.
+      exploit Memory.write_na_times; try exact WRITE_NA. i. des.
+      clear - ORD LOC MSG_EX ADD MEM2 WRITE_SRC x1.
+      inv MEM2. econs.
+      - etrans; eauto. ii.
+        erewrite Memory.add_o; eauto. condtac; ss; eauto. des. subst.
+        exploit Memory.add_get0; eauto. i. des. congr.
+      - i. revert GET_TGT. erewrite Memory.add_o; eauto.
+        condtac; ss; eauto. i. des. clarify.
+      - i. revert GET_TGT. erewrite Memory.add_o; eauto.
+        condtac; ss; eauto. i. des. clarify.
+        exploit Memory.write_get2; try exact WRITE_SRC. i. des.
+        right. esplits; eauto.
+        eapply TimeFacts.le_lt_lt; eauto.
+      - i. revert GET_TGT. erewrite Memory.add_o; eauto.
+        condtac; ss; eauto. i. des. clarify.
+        unguard. des; ss.
+    Qed.
+
+    Lemma promise_step
+          rels lc1_src mem1_src
+          lc1_tgt mem1_tgt loc from to msg lc2_tgt mem2_tgt kind
+          (LC1: lc1_src = lc1_tgt)
+          (MEM1: sim_memory rels mem1_src mem1_tgt)
+          (WRITES1: Writes.wf L rels mem1_src)
+          (WF1_SRC: Local.wf lc1_src mem1_src)
+          (STEP_TGT: Local.promise_step lc1_tgt mem1_tgt loc from to msg lc2_tgt mem2_tgt kind)
+          (MSG1: forall promises2_src mem2_src
+                   (PROMISE: Memory.promise (Local.promises lc1_src) mem1_src loc from to msg promises2_src mem2_src kind),
+              Memory.closed_message msg mem2_src):
+      exists lc2_src mem2_src,
+        (<<STEP_SRC: Local.promise_step lc1_src mem1_src loc from to msg lc2_src mem2_src kind>>) /\
+        (<<LC2: lc2_src = lc2_tgt>>) /\
+        (<<MEM2: sim_memory rels mem2_src mem2_tgt>>).
+    Proof.
+      inv STEP_TGT.
+      exploit promise; try exact MEM; eauto; try apply WF1_SRC; try apply WF1_TGT. i. des.
+      esplits; eauto.
+    Qed.
+
+    Lemma ordc_na
+          ordc ord loc
+          (ORDC: Ordering.le ordc Ordering.na):
+      (if L loc then Ordering.join ord ordc else ord) = ord.
+    Proof.
+      condtac; ss.
+      destruct ordc, ord; ss.
+    Qed.
+
+    Lemma read_step
+          rels lc1_src mem1_src
+          lc1_tgt mem1_tgt loc to val released ord lc2_tgt
+          (LC1: lc1_src = lc1_tgt)
+          (MEM1: sim_memory rels mem1_src mem1_tgt)
+          (WRITES1: Writes.wf L rels mem1_src)
+          (NORMAL_TVIEW1: Normal.normal_tview L (Local.tview lc1_src))
+          (NORMAL_MEM1: Normal.normal_memory L mem1_src)
+          (WF1_SRC: Local.wf lc1_src mem1_src)
+          (STEP_TGT: Local.read_step lc1_tgt mem1_tgt loc to val released ord lc2_tgt):
+      (exists lc2_src,
+          (<<STEP_SRC: OrdLocal.read_step L Ordering.na lc1_src mem1_src loc to val released ord lc2_src>>) /\
+          (<<LC2: lc2_src = lc2_tgt>>) /\
+          (<<NORMAL_TVIEW2: Normal.normal_tview L (Local.tview lc2_src)>>)) \/
+      (<<RACE: RARaceW.wr_race L rels (Local.tview lc1_src) loc ord>>).
+    Proof.
+      inv MEM1. inv STEP_TGT.
+      destruct (Memory.get loc to mem1_src) as [[from_src msg_src]|] eqn:GET_SRC; cycle 1.
+      { (* race *)
+        destruct (L loc) eqn:LOC; cycle 1.
+        { exploit COMPLETE1; eauto; try congr. }
+        inv READABLE. inv NORMAL_TVIEW1.
+        exploit COMPLETE2; eauto. i. des; try congr.
+        right. unfold RARaceW.wr_race.
+        esplits; try exact ORD0; eauto.
+        rewrite CUR; ss.
+      }
+      exploit SOUND; eauto. i. rewrite x in *. inv GET.
+      destruct (classic (L loc /\ Ordering.le ord Ordering.plain /\
+                         Time.lt (View.rlx (TView.cur (Local.tview lc1_tgt)) loc) to)).
+      { (* race *)
+        right. des. unfold RARaceW.wr_race.
+        inv WRITES1. exploit COMPLETE; try exact GET_SRC; eauto. i. des.
+        esplits; eauto.
+      }
+      left. esplits.
+      - econs; eauto. rewrite ordc_na; ss. eauto.
+      - ss.
+      - exploit Normal.read_step; try exact WF1_SRC; eauto. i.
+        inv READABLE. inv NORMAL_TVIEW1. rewrite CUR in *; ss.
+        inv PLN; ss.
+        exfalso. apply H. splits; ss.
+    Qed.
+
+    Lemma write_step
+          rels lc1_src sc1_src mem1_src
+          lc1_tgt sc1_tgt mem1_tgt loc from to val releasedm released ord lc2_tgt sc2_tgt mem2_tgt kind
+          (LC1: lc1_src = lc1_tgt)
+          (SC1: sc1_src = sc1_tgt)
+          (MEM1: sim_memory rels mem1_src mem1_tgt)
+          (WRITES1: Writes.wf L rels mem1_src)
+          (WF1_SRC: Local.wf lc1_src mem1_src)
+          (STEP_TGT: Local.write_step lc1_tgt sc1_tgt mem1_tgt loc from to val
+                                      releasedm released ord lc2_tgt sc2_tgt mem2_tgt kind):
+      exists lc2_src sc2_src mem2_src,
+        (<<STEP_SRC: OrdLocal.write_step L Ordering.plain
+                                         lc1_src sc1_src mem1_src loc from to val
+                                         releasedm released ord lc2_src sc2_src mem2_src kind>>) /\
+        (<<LC2: lc2_src = lc2_tgt>>) /\
+        (<<SC2: sc2_src = sc2_tgt>>) /\
+        (<<MEM2: sim_memory rels mem2_src mem2_tgt>>).
+    Proof.
+      inv STEP_TGT.
+      exploit write; try exact MEM1; eauto; try apply WF1_SRC. i. des.
+      esplits; eauto.
+      econs; eauto. econs; eauto; try (condtac; ss).
+      - unfold TView.write_released.
+        repeat condtac; destruct ord; ss.
+      - inv WRITABLE. econs. ss.
+      - destruct ord; ss.
+      - f_equal. unfold TView.write_released.
+        repeat condtac; destruct ord; ss.
+    Qed.
+
+    Lemma write_na_step_other
+          rels lc1_src sc1_src mem1_src
+          lc1_tgt sc1_tgt mem1_tgt loc from to val ord lc2_tgt sc2_tgt mem2_tgt msgs kinds kind
+          (LC1: lc1_src = lc1_tgt)
+          (SC1: sc1_src = sc1_tgt)
+          (MEM1: sim_memory rels mem1_src mem1_tgt)
+          (WRITES1: Writes.wf L rels mem1_src)
+          (WF1_SRC: Local.wf lc1_src mem1_src)
+          (LOC: ~ L loc)
+          (STEP_TGT: Local.write_na_step lc1_tgt sc1_tgt mem1_tgt loc from to val ord
+                                         lc2_tgt sc2_tgt mem2_tgt msgs kinds kind):
+      exists lc2_src sc2_src mem2_src,
+        (<<STEP_SRC: Local.write_na_step lc1_src sc1_src mem1_src loc from to val ord
+                                         lc2_src sc2_src mem2_src msgs kinds kind>>) /\
+        (<<LC2: lc2_src = lc2_tgt>>) /\
+        (<<SC2: sc2_src = sc2_tgt>>) /\
+        (<<MEM2: sim_memory rels mem2_src mem2_tgt>>).
+    Proof.
+      inv STEP_TGT.
+      exploit write_na_other; eauto; try apply WF1_SRC. i. des.
+      esplits; eauto.
+    Qed.
+
+    Lemma write_na_step_loc
+          rels lc1_src sc1_src mem1_src
+          lc1_tgt sc1_tgt mem1_tgt loc from to val ord lc2_tgt sc2_tgt mem2_tgt msgs kinds kind
+          (LC1: lc1_src = lc1_tgt)
+          (SC1: sc1_src = sc1_tgt)
+          (MEM1: sim_memory rels mem1_src mem1_tgt)
+          (WRITES1: Writes.wf L rels mem1_src)
+          (RESERVE_ONLY1: OrdLocal.reserve_only L (Local.promises lc1_src))
+          (WF1_SRC: Local.wf lc1_src mem1_src)
+          (LOC: L loc)
+          (STEP_TGT: Local.write_na_step lc1_tgt sc1_tgt mem1_tgt loc from to val ord
+                                         lc2_tgt sc2_tgt mem2_tgt msgs kinds kind):
+      exists lc2_src sc2_src mem2_src,
+        (<<STEP_SRC: OrdLocal.write_na_step L Ordering.plain
+                                            lc1_src sc1_src mem1_src loc from to val ord
+                                            lc2_src sc2_src mem2_src [] [] kind>>) /\
+        (<<LC2: lc2_src = lc2_tgt>>) /\
+        (<<SC2: sc2_src = sc2_tgt>>) /\
+        (<<MEM2: sim_memory ((loc, to, ord) :: rels) mem2_src mem2_tgt>>).
+    Proof.
+      inv STEP_TGT.
+      exploit write_na_loc; try exact MEM1; eauto; try apply WF1_SRC. i. des.
+      esplits; eauto. econs 2; eauto.
+      destruct (L loc); ss. econs; eauto.
+      - exploit Memory.write_na_times; eauto. i. des.
+        econs; eauto.
+      - unfold TView.write_released. condtac; eauto.
+        destruct ord; ss.
+      - destruct ord; ss.
+      - f_equal.
+        unfold TView.write_tview. f_equal.
+        repeat condtac; ss; destruct ord; ss.
+    Qed.
+
+    Lemma is_racy
+          rels lc1_src mem1_src
+          lc1_tgt mem1_tgt loc ord
+          (LC1: lc1_src = lc1_tgt)
+          (MEM1: sim_memory rels mem1_src mem1_tgt)
+          (NORMAL_TVIEW1: Normal.normal_tview L (Local.tview lc1_src))
+          (STEP_TGT: Local.is_racy lc1_tgt mem1_tgt loc ord):
+      (<<STEP_SRC: Local.is_racy lc1_src mem1_src loc ord>>) \/
+      (exists to ordw,
+          (<<LOC: L loc>>) /\
+          (<<HIGHER: Time.lt (View.rlx (TView.cur (Local.tview lc1_src)) loc) to>>) /\
+          (<<IN: List.In (loc, to, ordw) rels>>) /\
+          (<<ORD: Ordering.le ordw Ordering.na>>)).
+    Proof.
+      inv MEM1. inv STEP_TGT.
+      destruct (Memory.get loc to mem1_src) as [[from_src msg_src]|] eqn:GET_SRC.
+      { exploit SOUND; eauto. i.
+        rewrite x in *. inv GET. eauto.
+      }
+      destruct (L loc) eqn:LOC; cycle 1.
+      { exploit COMPLETE1; eauto. rewrite LOC. ss. }
+      exploit COMPLETE2; eauto.
+      { econs. eauto. }
+      i. des; eauto.
+      right. esplits; eauto.
+      inv NORMAL_TVIEW1. rewrite CUR; ss.
+    Qed.
+
+    Lemma racy_read_step
+          rels lc1_src mem1_src
+          lc1_tgt mem1_tgt loc val ord
+          (LC1: lc1_src = lc1_tgt)
+          (MEM1: sim_memory rels mem1_src mem1_tgt)
+          (NORMAL_TVIEW1: Normal.normal_tview L (Local.tview lc1_src))
+          (STEP_TGT: Local.racy_read_step lc1_tgt mem1_tgt loc val ord):
+      (<<STEP_SRC: OrdLocal.racy_read_step L Ordering.na lc1_src mem1_src loc val ord>>) \/
+      (<<RACE: RARaceW.wr_race L rels (Local.tview lc1_src) loc ord>>).
+    Proof.
+      inv STEP_TGT.
+      exploit is_racy; eauto. i. des.
+      - left. econs; eauto. rewrite ordc_na; ss.
+      - right. unfold RARaceW.wr_race.
+        esplits; eauto.
+    Qed.
+
+    Lemma racy_write_step
+          rels lc1_src mem1_src
+          lc1_tgt mem1_tgt loc ord
+          (LC1: lc1_src = lc1_tgt)
+          (MEM1: sim_memory rels mem1_src mem1_tgt)
+          (WRITES1: Writes.wf L rels mem1_src)
+          (NORMAL_TVIEW1: Normal.normal_tview L (Local.tview lc1_src))
+          (STEP_TGT: Local.racy_write_step lc1_tgt mem1_tgt loc ord):
+      (<<STEP_SRC: OrdLocal.racy_write_step L Ordering.plain lc1_src mem1_src loc ord>>) \/
+      (<<RACE: RARaceW.ww_race L rels (Local.tview lc1_src) loc ord>>).
+    Proof.
+      inv STEP_TGT.
+      exploit is_racy; eauto. i. des.
+      - destruct (L loc) eqn:LOC; cycle 1.
+        { left. econs; eauto. rewrite LOC. eauto. }
+        inv STEP_SRC. destruct msg; ss.
+        + inv WRITES1. exploit COMPLETE; eauto. i. des.
+          right. unfold RARaceW.ww_race.
+          inv NORMAL_TVIEW1. rewrite CUR; ss.
+          esplits; eauto. right.
+          destruct ord; ss; exploit MSG2; ss.
+        + left. econs; eauto.
+      - right. unfold RARaceW.ww_race.
+        esplits; eauto.
+    Qed.
+
+    Lemma racy_update_step
+          rels lc1_src mem1_src
+          lc1_tgt mem1_tgt loc ordr ordw
+          (LC1: lc1_src = lc1_tgt)
+          (MEM1: sim_memory rels mem1_src mem1_tgt)
+          (NORMAL_TVIEW1: Normal.normal_tview L (Local.tview lc1_src))
+          (STEP_TGT: Local.racy_update_step lc1_tgt mem1_tgt loc ordr ordw):
+      (<<STEP_SRC: Local.racy_update_step lc1_src mem1_src loc ordr ordw>>) \/
+      (<<RACE: RARaceW.ww_race L rels (Local.tview lc1_src) loc ordw>>).
+    Proof.
+      inv STEP_TGT; eauto.
+      exploit is_racy; eauto. i. des; eauto.
+      right. unfold RARaceW.ww_race.
+      esplits; eauto.
+    Qed.
+
+    Variant sim_event: forall (e_src e_tgt: ThreadEvent.t), Prop :=
+    | sim_event_promise
+        loc from to msg kind:
+        sim_event (ThreadEvent.promise loc from to msg kind)
+                  (ThreadEvent.promise loc from to msg kind)
+    | sim_event_silent:
+        sim_event ThreadEvent.silent ThreadEvent.silent
+    | sim_event_read
+        loc to val released ord:
+        sim_event (ThreadEvent.read loc to val released ord)
+                  (ThreadEvent.read loc to val released ord)
+    | sim_event_write
+        loc from to val released ord:
+        sim_event (ThreadEvent.write loc from to val released ord)
+                  (ThreadEvent.write loc from to val released ord)
+    | sim_event_write_na
+        loc msgs_src msgs_tgt from to val ord:
+        sim_event (ThreadEvent.write_na loc msgs_src from to val ord)
+                  (ThreadEvent.write_na loc msgs_tgt from to val ord)
+    | sim_event_update
+        loc from to valr valw releasedm released ordr ordw:
+        sim_event (ThreadEvent.update loc from to valr valw releasedm released ordr ordw)
+                  (ThreadEvent.update loc from to valr valw releasedm released ordr ordw)
+    | sim_event_fence
+        ordr ordw:
+        sim_event (ThreadEvent.fence ordr ordw) (ThreadEvent.fence ordr ordw)
+    | sim_event_syscall
+        e:
+        sim_event (ThreadEvent.syscall e) (ThreadEvent.syscall e)
+    | sim_event_failure:
+      sim_event ThreadEvent.failure ThreadEvent.failure
+    | sim_event_racy_read
+        loc val ord:
+      sim_event (ThreadEvent.racy_read loc val ord)
+                (ThreadEvent.racy_read loc val ord)
+    | sim_event_racy_write
+        loc val ord:
+      sim_event (ThreadEvent.racy_write loc val ord)
+                (ThreadEvent.racy_write loc val ord)
+    | sim_event_racy_update
+        loc valr valw ordr ordw:
+      sim_event (ThreadEvent.racy_update loc valr valw ordr ordw)
+                (ThreadEvent.racy_update loc valr valw ordr ordw)
+    .
+    Hint Constructors sim_event.
+
+    Lemma program_step
+          rels lc1_src sc1_src mem1_src
+          e_tgt lc1_tgt sc1_tgt mem1_tgt lc2_tgt sc2_tgt mem2_tgt
+          (LC1: lc1_src = lc1_tgt)
+          (SC1: sc1_src = sc1_tgt)
+          (MEM1: sim_memory rels mem1_src mem1_tgt)
+          (WRITES1: Writes.wf L rels mem1_src)
+          (RESERVE_ONLY1: OrdLocal.reserve_only L (Local.promises lc1_src))
+          (NORMAL_TVIEW1: Normal.normal_tview L (Local.tview lc1_src))
+          (NORMAL_MEM1: Normal.normal_memory L mem1_src)
+          (WF1_SRC: Local.wf lc1_src mem1_src)
+          (SC1_SRC: Memory.closed_timemap sc1_src mem1_src)
+          (MEM1_SRC: Memory.closed mem1_src)
+          (STEP_TGT: Local.program_step e_tgt lc1_tgt sc1_tgt mem1_tgt lc2_tgt sc2_tgt mem2_tgt):
+      (exists e_src lc2_src sc2_src mem2_src,
+          (<<STEP_SRC: OrdLocal.program_step L Ordering.na Ordering.plain 
+                                             e_src lc1_src sc1_src mem1_src lc2_src sc2_src mem2_src>>) /\
+          (<<EVENT: sim_event e_src e_tgt>>) /\
+          (<<LC2: lc2_src = lc2_tgt>>) /\
+          (<<SC2: sc2_src = sc2_tgt>>) /\
+          (<<MEM2: sim_memory (Writes.append L e_src rels) mem2_src mem2_tgt>>) /\
+          (<<NORMAL_TVIEW2: Normal.normal_tview L (Local.tview lc2_src)>>) /\
+          (<<NORMAL_MEM2: Normal.normal_memory L mem2_src>>)) \/
+      (<<RACE: RARaceW.ra_race L rels (Local.tview lc1_src) (ThreadEvent.get_program_event e_tgt)>>).
+    Proof.
+      inv STEP_TGT.
+      - left. esplits; eauto. econs.
+      - exploit read_step; eauto. i. des.
+        + left. esplits; eauto. econs. ss.
+        + right. left. ss. esplits; eauto.
+      - exploit write_step; eauto. i. des.
+        dup STEP_SRC. inv STEP_SRC0.
+        exploit Normal.write_step; try exact STEP; eauto; ss. i. des.
+        left. esplits; [econs 3|..]; eauto.
+        eapply sim_memory_append; eauto.
+      - exploit read_step; eauto. i. des; cycle 1.
+        { right. left. esplits; ss; eauto. }
+        dup STEP_SRC. inv STEP_SRC0.
+        exploit Local.read_step_future; try exact STEP; eauto. i. des.
+        exploit write_step; eauto. i. des.
+        dup STEP_SRC0. inv STEP_SRC1.
+        exploit Normal.write_step; try exact STEP0; eauto.
+        { inv STEP. destruct releasedr; ss. eauto. }
+        i. des.
+        left. esplits; [econs 4|..]; eauto.
+        eapply sim_memory_append; eauto.
+      - left. esplits; [econs 5|..]; eauto.
+        exploit Normal.fence_step; eauto.
+      - left. esplits; [econs 6|..]; eauto.
+        exploit Normal.fence_step; eauto.
+      - left. esplits; [econs 7|..]; eauto.
+      - destruct (L loc) eqn:LOC.
+        + exploit write_na_step_loc; try exact LOCAL; eauto. i. des.
+          exploit (@Normal.ord_program_step L Ordering.na Ordering.plain);
+            try econs 8; eauto; ss. i. des.
+          left. esplits; [econs 8|..]; eauto.
+          unfold Writes.append. ss. condtac; ss.
+        + exploit write_na_step_other; try exact LOCAL; eauto; try congr. i. des.
+          exploit Normal.write_na_step; try exact STEP_SRC; eauto. i. des.
+          left. esplits; [econs 8|..]; eauto.
+          * econs; eauto. condtac; ss. eauto.
+          * unfold Writes.append. ss. condtac; ss.
+      - exploit racy_read_step; try exact LOCAL; eauto. i. des.
+        + left. esplits; [econs 9|..]; eauto.
+        + right. left. esplits; ss; eauto.
+      - exploit racy_write_step; try exact LOCAL; eauto. i. des.
+        + left. esplits; [econs 10|..]; eauto.
+        + right. right. esplits; ss; eauto.
+      - exploit racy_update_step; try exact LOCAL; eauto. i. des.
+        + left. esplits; [econs 11|..]; eauto.
+        + right. right. esplits; ss; eauto.
+    Qed.
   End PFtoAPFSimThread.
 End PFtoAPFSimThread.
